src/spec/notations.v
@@ -1,0 +1,24 @@
+From mathcomp
+     Require Import ssreflect ssrbool eqtype ssrnat seq fintype ssrfun
+                    tuple finset.
+From CoqEAL
+     Require Import refinements.
+Require Import ops spec spec.operations.
+
+Import Refinements.Op.
+Import Logical.Op.
+
+Global Instance eq_Bits {n} : eq_of (BITS n) := fun x y => x == y.
+Global Instance one_Bits {n} : one_of (BITS n) := #1.
+Global Instance zero_Bits {n} : zero_of (BITS n) := @zero n.
+
+Definition sub {n} (x y : BITS n): BITS n := subB x y.
+
+Global Instance sub_Bits {n} : sub_of (BITS n) := sub.
+
+Global Instance not_Bits {n} : not_of (BITS n) := @invB n.
+Global Instance or_Bits {n} : or_of (BITS n) := @orB n.
+Global Instance and_Bits {n} : and_of (BITS n) := @andB n.
+Global Instance xor_Bits {n} : xor_of (BITS n) := @xorB n.
+Global Instance shr_Bits {n} : shr_of (BITS n) := (fun x y => @shrBn n x (toNat y)).
+Global Instance shl_Bits {n} : shl_of (BITS n) := (fun x y => @shlBn n x (toNat y)).
